thys/JinjaThreads/Common/SemiType.thy
@@ -458,7 +458,7 @@ proof -
       qed
     qed }
   with is_class_Object[OF wf] sup itA itB show ?thesis unfolding sup_def
-    by(cases "A = B")(auto split: split_if_asm simp add: mem_def exec_lub_refl)
+    by(cases "A = B")(auto split: split_if_asm simp add: exec_lub_refl)
 qed
 
 lemma closed_err_types:
@@ -505,7 +505,7 @@ proof -
       using acyclic_widen1[OF wfP] superI[of _ _ P]
       by(simp add: exec_lub_conv)(blast dest: is_lubD is_ubD intro: widen1_rtrancl_into_widen) }
   with it1 it2 sup show ?thesis
-    by(cases s, auto simp add: sup_def split: split_if_asm elim: refTE)
+    by (cases s) (auto simp add: sup_def split: split_if_asm elim: refTE)
 qed
 
 lemma sup_widen_smallest:
@@ -613,9 +613,10 @@ lemma eval_widen1p_i_i_o_conv:
 by(auto elim: widen1p_i_i_oE intro: widen1p_i_i_oI simp add: widen1_def fun_eq_iff)
 
 lemma rtrancl_widen1_code [code_unfold]:
-  "(widen1 P)^* = (\<lambda>(a, b). Predicate.holds (rtrancl_tab_FioB_i_i_i (widen1p_i_i_o P) [] a b))"
-by(auto simp add: fun_eq_iff Predicate.holds_eq widen1_def Collect_def rtrancl_def mem_def rtranclp_eq_rtrancl_tab_nil eval_widen1p_i_i_o_conv intro!: rtrancl_tab_FioB_i_i_iI elim!: rtrancl_tab_FioB_i_i_iE)
+  "(widen1 P)^* = {(a, b). Predicate.holds (rtrancl_tab_FioB_i_i_i (widen1p_i_i_o P) [] a b)}"
+by(auto simp add: fun_eq_iff Predicate.holds_eq widen1_def rtrancl_def rtranclp_eq_rtrancl_tab_nil eval_widen1p_i_i_o_conv intro!: rtrancl_tab_FioB_i_i_iI elim!: rtrancl_tab_FioB_i_i_iE)
 
 declare exec_lub_def [code_unfold]
 
 end
+
