thys/JinjaThreads/Framework/FWSemantics.thy
@@ -334,7 +334,7 @@ lemma redT_ex_new_thread':
 using assms
 by(cases)(fastforce split: split_if_asm dest!: redT_updTs_new_thread)+
 
-definition deterministic :: "(('l,'t,'x,'m,'w) state \<Rightarrow> bool) \<Rightarrow> bool"
+definition deterministic :: "('l,'t,'x,'m,'w) state set \<Rightarrow> bool"
 where
   "deterministic I \<longleftrightarrow> 
   (\<forall>s t x ta' x' m' ta'' x'' m''. 
